---
tags:
  - maths
  - physics
---

Any function can be decomposed into a sum of even and odd functions

$$
f(x) = \dfrac{1}{2}[f(x) + f(-x)] + \dfrac{1}{2}[f(x)-f(-x)]
$$

We define

$$
\sinh(x) = \dfrac{1}{2}(e^x - e^{-x})
$$
$$
\cosh(x) =  \dfrac{1}{2}(e^x + e^{-x})
$$

Properties:
- $\cosh^2x - \sinh^2x =1$
- $\cosh (a+b) = \cosh a \cosh b - \sinh a \sinh b$
- $\sinh (a+b) = \sinh a \cosh b - \cosh a \sinh b$

### Hyperbolic trigonometry 
$$
x^2 - y^2 = 1 \quad \Rightarrow \quad \cosh^2t - \sinh^2t = 1
$$
